One slow example

src/Examples/Locks.v
@@ -30,6 +30,12 @@ Module Locks.
 
   Definition S (n : nat) := Vector.t bool n.
 
+  Fixpoint init (n : nat) : S n :=
+    match n with
+    | O => Vector.nil bool
+    | Datatypes.S n => Vector.cons bool false n (init n)
+    end.
+
   Definition m (n : nat) : Model.t (E n) (S n) :=
     fun c s =>
       match c with
@@ -38,12 +44,54 @@ Module Locks.
         if b then
           None
         else
-          Some (tt, Vector.replace s id false)
+          Some (tt, Vector.replace s id true)
       | Command.Unlock id =>
         let b := Vector.nth s id in
         if b then
-          Some (tt, Vector.replace s id true)
+          Some (tt, Vector.replace s id false)
         else
           None
       end.
 End Locks.
+
+Definition ex1 : C.t (Locks.E 1) nat :=
+  do! Locks.lock Fin.F1 in
+  do! Locks.unlock Fin.F1 in
+  ret 12.
+
+Lemma ex1_ok : C.DeadLockFree.t (Locks.m 1) (Locks.init 1) ex1.
+  now apply Decide.C.dead_lock_free_ok.
+Qed.
+
+Fixpoint iter_seq {n : nat} (l : list (C.t (Locks.E n) unit))
+  : C.t (Locks.E n) unit :=
+  match l with
+  | [] => ret tt
+  | x :: l => do! x in iter_seq l
+  end.
+
+Fixpoint iter_par {n : nat} (l : list (C.t (Locks.E n) unit))
+  : C.t (Locks.E n) unit :=
+  match l with
+  | [] => ret tt
+  | x :: l =>
+    let! _ : unit * unit := join x (iter_par l) in
+    ret tt
+  end.
+
+Definition ex2 : C.t (Locks.E 3) unit :=
+  let a : Fin.t 3 := Fin.F1 in
+  let b : Fin.t 3 := Fin.FS Fin.F1 in
+  let c : Fin.t 3 := Fin.FS (Fin.FS Fin.F1) in
+  iter_par (List.map iter_seq [
+    [Locks.lock a; Locks.lock c; Locks.unlock c; Locks.unlock a];
+    [Locks.lock a; Locks.lock c; Locks.unlock c; Locks.unlock a];
+    [Locks.lock b; Locks.lock c; Locks.unlock c; Locks.unlock b];
+    [Locks.lock b; Locks.lock c; Locks.unlock c; Locks.unlock b]]).
+
+Time Compute Decide.dead_lock_free (Locks.m 3) (Locks.init 3)
+  (Compile.to_choose ex2).
+
+Lemma ex2_ok : C.DeadLockFree.t (Locks.m 3) (Locks.init 3) ex2.
+  now apply Decide.C.dead_lock_free_ok.
+Qed.
